@prefix otl: <https://w3id.org/opentrafficlights#> .
@prefix rdf: <http://www.w3.org/1999/02/22-rdf-syntax-ns#> .
@prefix foaf: <http://xmlns.com/foaf/0.1/> .
@prefix dct: <http://purl.org/dc/terms/> .
@prefix rdfs: <http://www.w3.org/2000/01/rdf-schema#> .
@prefix owl: <http://www.w3.org/2002/07/owl#> .
@prefix xsd: <http://www.w3.org/2001/XMLSchema#> .
@prefix vann: <http://purl.org/vocab/vann/> .
@prefix skos: <http://www.w3.org/2004/02/skos/core#> .
@prefix otl: <https://w3id.org/opentrafficlights#> .
@prefix dcat: <http://www.w3.org/ns/dcat#> .

<https://w3id.org/opentrafficlights> a foaf:Document ;
                                              foaf:primaryTopic lc:Ontology ;
                                              dct:issued "2018-06-20"^^xsd:date ;
                                              dct:modified "2018-10-30"^^xsd:date ;
                                              dct:license <http://creativecommons.org/licenses/by/3.0/> .

otl:Ontology a owl:Ontology ;
            rdfs:label "The Open Traffic Lights ontology"@en ;
            rdfs:comment "This ontology provides the terms necessary to describe the status of traffic lights."@en ;
            vann:preferredNamespacePrefix "otl" ;
            vann:preferredNamespaceUri "https://w3id.org/opentrafficlights#" ;
            dct:creator <https://w3id.org/people/brechtvdv/#me> .
            
otl:Lane a rdfs:Class ;
              rdfs:label "Lane"@en ;
              rdfs:comment "Describes a part of the road where a passenger departs or arrives from."@en .

otl:width a rdf:Property ;
               rdfs:label "Width"@en ;
               rdfs:comment "The width of a lane expressed in centimeters."@en ;
               rdfs:domain otl:Lane;
               rdfs:range xsd:Integer .

otl:Connection a rdfs:Class ;
              rdfs:label "Connection"@en ;
              rdfs:comment "Describes a departure at a certain lane and an arrival at a different lane"@en .

otl:departureLane a rdf:Property ;
               rdfs:label "Departure lane"@en ;
               rdfs:comment "A road user will depart from here"@en ;
               rdfs:domain otl:Connection .
               
otl:arrivalLane a rdf:Property ;
               rdfs:label "Arrival lane"@en ;
               rdfs:comment "A road user will arrive here"@en ;
               rdfs:domain otl:Connection .

otl:Signalgroup a rdfs:Class ;
              rdfs:label "Signal group"@en ;
              rdfs:comment "Describes a group of traffic lights by having the same event state."@en .
              
otl:EventState a rdfs:Class ;
              rdfs:label "Event state"@en ;
              rdfs:comment "Describes the state of a signal group."@en .
              
otl:eventState a rdf:Property ;
               rdfs:label "Event state"@en ;
               rdfs:comment "Event state of a signal group."@en ;
               rdfs:domain otl:Signalgroup ;
               rdfs:range otl:EventState .
               
otl:minEndTime a rdf:Property ;
               rdfs:label "Minimum end time"@en ;
               rdfs:comment "The earliest time possible at which the event state could change, except when unpredictable events relating to a pre-emption or priority call disrupt a currently active timing plan.
"@en ;
               rdfs:domain otl:EventState ;
               rdfs:range xsd:dateTime .
               
otl:maxEndTime a rdf:Property ;
               rdfs:label "Maximum end time"@en ;
               rdfs:comment "The latest time possible at which the event state could change, except when unpredictable events relating to a pre-emption or priority call disrupt a currently active timing plan.
"@en ;
               rdfs:domain otl:EventState ;
               rdfs:range xsd:dateTime .
